bce/bce_proof.dfy
@@ -63,6 +63,15 @@ lemma lemma_BCE_Validity(s:Service, s':Service, s'':Service)
     lemma_BCE_Validity_Correct_Nodes_Send_Good_Syndrome(s'); 
     var syndromes := syndromesToExchange(s'.nodes);
     lemma_Exchanged_Syndromes_Are_Extracted(s'.nodes);
+    forall node | node in s'.nodes && !node.faulty  
+    ensures forall syn :: syn in syndromes[node.id] ==> |syn| == s'.n
+    {
+        assert syndromes[node.id] == extractSyndromes(s'.nodes);
+        lemma_Extract_Generates_One_Syndrome_For_Each_Node(s'.nodes);
+        assert forall i :: 0 <= i < |s'.nodes| ==> syndromes[node.id][i] == computeSyndrome(s'.nodes[i]);
+    }
+    assert forall node :: node in s'.nodes && !node.faulty ==>
+        (forall syn :: syn in syndromes[node.id] ==> |syn| == s'.n);
     lemma_BCE_Validity_Correct_Nodes_Decide_Codeword(s', syndromes);
 }
 
@@ -223,6 +232,8 @@ lemma lemma_BCE_Validity_Correct_Nodes_Decide_Codeword(s':Service, syndromes: se
         && nd.state == Phase2
         && 0 <= nd.id < s'.n
         && 0 <= nd.id < |syndromes[nd.id]|;
+    requires forall node :: node in s'.nodes && !node.faulty ==>
+        (forall syn :: syn in syndromes[node.id] ==> |syn| == s'.n);
     // Facts needed for this proof
     requires forall id :: 0 <= id < s'.n 
         ==> 
@@ -247,131 +258,132 @@ lemma lemma_BCE_Validity_Correct_Nodes_Decide_Codeword(s':Service, syndromes: se
         assert countTrue(my_syndrome) >= node.n - node.f;
 
         // Prove that n-f of received syndromes are good
-        assert forall i :: 0 <= i < s'.n ==> syndromes_received[i] == computeSyndrome(s'.nodes[i]);
-        lemma_BCE_Validity_CountGoodSyndromes_Succeeds(s', node, syndromes_received);
+        // assert forall i :: 0 <= i < s'.n ==> syndromes_received[i] == computeSyndrome(s'.nodes[i]);
+        // lemma_BCE_Validity_CountGoodSyndromes_Succeeds(s', node, syndromes_received);
+        // TODO
     }
 }
 
 
 
 /* Prove that if node is correct, then countGoodSyndromes will give a count >= n-f */
-lemma {:induction syndromes_received} lemma_BCE_Validity_CountGoodSyndromes_Succeeds(s':Service, node: Node, syndromes_received: seq<syndrome>) 
-    // Boilerplate stuff
-    requires node_invariants(s');
-    requires |s'.nodes| == s'.n;
-    requires forall  i :: 0 <= i < s'.n ==> s'.nodes[i].id == i
-    requires node in s'.nodes;
-    requires forall n :: n in s'.nodes ==> n.n == |n.symbols| == |n.codeword|;
-    requires |syndromesToExchange(s'.nodes)| == s'.n;
-    requires syndromes_received == syndromesToExchange(s'.nodes)[node.id];
-    requires |syndromes_received| == s'.n;
-    requires forall i :: 0 <= i < s'.n ==> syndromes_received[i] == computeSyndrome(s'.nodes[i]);
-    requires forall nd :: 
-        nd in s'.nodes && !nd.faulty
-        ==>
-        && nd.state == Phase2
-        && 0 <= nd.id < s'.n
-    // Facts needed for this proof
-    requires forall id :: 0 <= id < s'.n 
-        ==> 
-        (!s'.nodes[id].faulty ==> countTrue(computeSyndrome(s'.nodes[id])) >= s'.n - s'.f);
-    requires forall node1, node2 :: 
-            && node1 in s'.nodes && node2 in s'.nodes 
-            && !node1.faulty && !node2.faulty ==> 
-            node1.codeword == node2.codeword;
-    requires countFaulty(s'.nodes) <= s'.f;
-    ensures countGoodSyndromes(syndromes_received, node.n-node.f) >= s'.n - s'.f;
-{
-    assert s'.nodes[..s'.n] == s'.nodes;
-    assert countFaulty(s'.nodes[..s'.n]) <= s'.f;
-    lemma_BCE_Validity_CountGoodSyndromes_Succeeds_Helper(s', node, syndromes_received, s'.n, s'.f);
-    assert syndromes_received[..s'.n] == syndromes_received;
-}
+// lemma {:induction syndromes_received} lemma_BCE_Validity_CountGoodSyndromes_Succeeds(s':Service, node: Node, syndromes_received: seq<syndrome>) 
+//     // Boilerplate stuff
+//     requires node_invariants(s');
+//     requires |s'.nodes| == s'.n;
+//     requires forall  i :: 0 <= i < s'.n ==> s'.nodes[i].id == i
+//     requires node in s'.nodes;
+//     requires forall n :: n in s'.nodes ==> n.n == |n.symbols| == |n.codeword|;
+//     requires |syndromesToExchange(s'.nodes)| == s'.n;
+//     requires syndromes_received == syndromesToExchange(s'.nodes)[node.id];
+//     requires |syndromes_received| == s'.n;
+//     requires forall i :: 0 <= i < s'.n ==> syndromes_received[i] == computeSyndrome(s'.nodes[i]);
+//     requires forall nd :: 
+//         nd in s'.nodes && !nd.faulty
+//         ==>
+//         && nd.state == Phase2
+//         && 0 <= nd.id < s'.n
+//     // Facts needed for this proof
+//     requires forall id :: 0 <= id < s'.n 
+//         ==> 
+//         (!s'.nodes[id].faulty ==> countTrue(computeSyndrome(s'.nodes[id])) >= s'.n - s'.f);
+//     requires forall node1, node2 :: 
+//             && node1 in s'.nodes && node2 in s'.nodes 
+//             && !node1.faulty && !node2.faulty ==> 
+//             node1.codeword == node2.codeword;
+//     requires countFaulty(s'.nodes) <= s'.f;
+//     ensures countGoodSyndromes(syndromes_received, node.n-node.f) >= s'.n - s'.f;
+// {
+//     assert s'.nodes[..s'.n] == s'.nodes;
+//     assert countFaulty(s'.nodes[..s'.n]) <= s'.f;
+//     lemma_BCE_Validity_CountGoodSyndromes_Succeeds_Helper(s', node, syndromes_received, s'.n, s'.f);
+//     assert syndromes_received[..s'.n] == syndromes_received;
+// }
 
 
-lemma {:induction i, f} lemma_BCE_Validity_CountGoodSyndromes_Succeeds_Helper(s':Service, node: Node, syndromes_received: seq<syndrome>, i: int, f: int) 
-    decreases i, f;
-    // Boilerplate stuff
-    requires node_invariants(s');
-    requires |s'.nodes| == s'.n;
-    requires forall  id :: 0 <= id < s'.n ==> s'.nodes[id].id == id
-    requires node in s'.nodes;
-    requires forall n :: n in s'.nodes ==> n.n == |n.symbols| == |n.codeword|;
-    requires |syndromesToExchange(s'.nodes)| == s'.n;
-    requires syndromes_received == syndromesToExchange(s'.nodes)[node.id];
-    requires |syndromes_received| == s'.n;
-    requires forall id :: 0 <= id < s'.n ==> syndromes_received[id] == computeSyndrome(s'.nodes[id]);
-    // Facts needed for this proof
-    requires forall id :: 0 <= id < s'.n ==> 
-        (!s'.nodes[id].faulty ==> countTrue(computeSyndrome(s'.nodes[id])) >= s'.n - s'.f)
-    requires 0 <= i <= s'.n;
-    requires 0 <= f <= s'.f;
-    requires countFaulty(s'.nodes[..i]) <= f;
-    ensures countGoodSyndromes(syndromes_received[..i], node.n-node.f) >= i - f;
-{
-    var thresh := s'.n - s'.f;
-    if i == 0 {
-        assert countGoodSyndromes(syndromes_received[..i], thresh) == 0;
-    } else { // Check the next syndrome (ith) for goodness
-        if !s'.nodes[i-1].faulty {
-            // If node is correct:
-            // Check countFaulty
-            lemma_Count_Faulty_Increment_Property(s'.nodes, i);
+// lemma {:induction i, f} lemma_BCE_Validity_CountGoodSyndromes_Succeeds_Helper(s':Service, node: Node, syndromes_received: seq<syndrome>, i: int, f: int) 
+//     decreases i, f;
+//     // Boilerplate stuff
+//     requires node_invariants(s');
+//     requires |s'.nodes| == s'.n;
+//     requires forall  id :: 0 <= id < s'.n ==> s'.nodes[id].id == id
+//     requires node in s'.nodes;
+//     requires forall n :: n in s'.nodes ==> n.n == |n.symbols| == |n.codeword|;
+//     requires |syndromesToExchange(s'.nodes)| == s'.n;
+//     requires syndromes_received == syndromesToExchange(s'.nodes)[node.id];
+//     requires |syndromes_received| == s'.n;
+//     requires forall id :: 0 <= id < s'.n ==> syndromes_received[id] == computeSyndrome(s'.nodes[id]);
+//     // Facts needed for this proof
+//     requires forall id :: 0 <= id < s'.n ==> 
+//         (!s'.nodes[id].faulty ==> countTrue(computeSyndrome(s'.nodes[id])) >= s'.n - s'.f)
+//     requires 0 <= i <= s'.n;
+//     requires 0 <= f <= s'.f;
+//     requires countFaulty(s'.nodes[..i]) <= f;
+//     ensures countGoodSyndromes(syndromes_received[..i], node.n-node.f) >= i - f;
+// {
+//     var thresh := s'.n - s'.f;
+//     if i == 0 {
+//         assert countGoodSyndromes(syndromes_received[..i], thresh) == 0;
+//     } else { // Check the next syndrome (ith) for goodness
+//         if !s'.nodes[i-1].faulty {
+//             // If node is correct:
+//             // Check countFaulty
+//             lemma_Count_Faulty_Increment_Property(s'.nodes, i);
 
-            // Invoke induction hypothesis
-            lemma_BCE_Validity_CountGoodSyndromes_Succeeds_Helper(s', node, syndromes_received, i-1, f);
+//             // Invoke induction hypothesis
+//             lemma_BCE_Validity_CountGoodSyndromes_Succeeds_Helper(s', node, syndromes_received, i-1, f);
 
-            // Check countGoodSyndromes
-            var check_prefix := syndromes_received[..i];
-            var x := countTrue(check_prefix[|check_prefix|-1]);
-            assert x >= thresh;
-            assert countGoodSyndromes(check_prefix, thresh) ==
-                1 + countGoodSyndromes(check_prefix[..|check_prefix|-1], thresh);
-            assert check_prefix[..|check_prefix|-1] == syndromes_received[..i-1];
-        } else {
-            // If node is faulty:
-            if f > 0 {
-                // Check countFaulty
-                lemma_Count_Faulty_Increment_Property(s'.nodes, i);
-                assert countFaulty(s'.nodes[..i-1]) == countFaulty(s'.nodes[..i]) - 1;
+//             // Check countGoodSyndromes
+//             var check_prefix := syndromes_received[..i];
+//             var x := countTrue(check_prefix[|check_prefix|-1]);
+//             assert x >= thresh;
+//             assert countGoodSyndromes(check_prefix, thresh) ==
+//                 1 + countGoodSyndromes(check_prefix[..|check_prefix|-1], thresh);
+//             assert check_prefix[..|check_prefix|-1] == syndromes_received[..i-1];
+//         } else {
+//             // If node is faulty:
+//             if f > 0 {
+//                 // Check countFaulty
+//                 lemma_Count_Faulty_Increment_Property(s'.nodes, i);
+//                 assert countFaulty(s'.nodes[..i-1]) == countFaulty(s'.nodes[..i]) - 1;
 
-                // Invoke induction hypothesis
-                lemma_BCE_Validity_CountGoodSyndromes_Succeeds_Helper(s', node, syndromes_received, i-1, f-1);
+//                 // Invoke induction hypothesis
+//                 lemma_BCE_Validity_CountGoodSyndromes_Succeeds_Helper(s', node, syndromes_received, i-1, f-1);
 
-                // Check countGoodSyndromes
-                var check_prefix := syndromes_received[..i];
-                var x := countTrue(check_prefix[|check_prefix|-1]);
-                if x >= thresh {
-                    assert countGoodSyndromes(check_prefix, thresh) ==
-                        1 + countGoodSyndromes(check_prefix[..|check_prefix|-1], thresh);
-                    assert check_prefix[..|check_prefix|-1] == syndromes_received[..i-1];
-                } else {
-                    assert countGoodSyndromes(check_prefix, thresh) == countGoodSyndromes(check_prefix[..|check_prefix|-1], thresh);
-                    assert check_prefix[..|check_prefix|-1] == syndromes_received[..i-1];
-                }
-            } else {
-                // f=0, so every node seen must be correct from this point. 
-                if !s'.nodes[i-1].faulty {
-                    lemma_BCE_Validity_CountGoodSyndromes_Succeeds_Helper(s', node, syndromes_received, i-1, f);
-                    var check_prefix := syndromes_received[..i];
-                    var x := countTrue(check_prefix[|check_prefix|-1]);
-                    assert x >= thresh;
-                    assert countGoodSyndromes(check_prefix, thresh) ==
-                        1 + countGoodSyndromes(check_prefix[..|check_prefix|-1], thresh);
-                    assert check_prefix[..|check_prefix|-1] == syndromes_received[..i-1];
-                } else {
-                    // Proof by contradiction that s'.nodes[i-1] cannot be faulty
-                    assert f == 0;
-                    assert countFaulty(s'.nodes[..i]) <= f;
-                    lemma_Count_Faulty_Increment_Property(s'.nodes, i);
-                    assert countFaulty(s'.nodes[..i-1]) < 0;
-                    lemma_Count_Faulty_Non_Negative_Property(s'.nodes[..i-1]);
-                    assert false; // Contradiction!
-                }
-            }
-        }
-    }
-}
+//                 // Check countGoodSyndromes
+//                 var check_prefix := syndromes_received[..i];
+//                 var x := countTrue(check_prefix[|check_prefix|-1]);
+//                 if x >= thresh {
+//                     assert countGoodSyndromes(check_prefix, thresh) ==
+//                         1 + countGoodSyndromes(check_prefix[..|check_prefix|-1], thresh);
+//                     assert check_prefix[..|check_prefix|-1] == syndromes_received[..i-1];
+//                 } else {
+//                     assert countGoodSyndromes(check_prefix, thresh) == countGoodSyndromes(check_prefix[..|check_prefix|-1], thresh);
+//                     assert check_prefix[..|check_prefix|-1] == syndromes_received[..i-1];
+//                 }
+//             } else {
+//                 // f=0, so every node seen must be correct from this point. 
+//                 if !s'.nodes[i-1].faulty {
+//                     lemma_BCE_Validity_CountGoodSyndromes_Succeeds_Helper(s', node, syndromes_received, i-1, f);
+//                     var check_prefix := syndromes_received[..i];
+//                     var x := countTrue(check_prefix[|check_prefix|-1]);
+//                     assert x >= thresh;
+//                     assert countGoodSyndromes(check_prefix, thresh) ==
+//                         1 + countGoodSyndromes(check_prefix[..|check_prefix|-1], thresh);
+//                     assert check_prefix[..|check_prefix|-1] == syndromes_received[..i-1];
+//                 } else {
+//                     // Proof by contradiction that s'.nodes[i-1] cannot be faulty
+//                     assert f == 0;
+//                     assert countFaulty(s'.nodes[..i]) <= f;
+//                     lemma_Count_Faulty_Increment_Property(s'.nodes, i);
+//                     assert countFaulty(s'.nodes[..i-1]) < 0;
+//                     lemma_Count_Faulty_Non_Negative_Property(s'.nodes[..i-1]);
+//                     assert false; // Contradiction!
+//                 }
+//             }
+//         }
+//     }
+// }
 
 
 /* Prove that for any correct node, its own syndrome has n-f 'true' bits */
